project/inductive/basic/inductive_graph_basic_theory.v
@@ -12,6 +12,8 @@ Import ListNotations.
 Require Import FSets.
 Require Import FMaps.
 Require Import OrderedTypeEx.
+Require Import Setoid Morphisms.
+
 
 Require Import MyProject.project.util.NatSet.
 
@@ -25,14 +27,8 @@ Require Import MyProject.project.relational_graph_theory.
 
 
 (* Section to make rewrite work with IG_equiv *)
-
-
-
-(* Source for rewrite: https://stackoverflow.com/questions/56099646/use-rewrite-tactic-with-my-own-operator-in-coq *)
-Require Import Setoid Morphisms.
-(* TODO: this could be made generic *)
 (* This proof is based on === being an equivalence relation *)
-Instance IG_Equivalence_eq : Equivalence IG_equiv.
+Instance IG_Equivalence_eq : Equivalence IG_basic_equiv.
 Proof.
   G_derived_equivalence_prover nat IG_basic_to_RG.
 Qed.
@@ -81,10 +77,10 @@ Qed.
 
 (* This is the most useful one for proving other statements.
   Use it to convert from "use friendly" In- statements to "provable" NatMap.In- statements  *)
-Lemma In_labNodes_is_InMap : forall (x : Node) (ig : IG),
-  In x (labNodes ig) <-> NatMap.In x ig.
+Lemma In_labNodes_is_InMap : forall (x : Node) (ig : IG_basic),
+  In x (IG_basic_labNodes ig) <-> NatMap.In x ig.
 Proof.
-  intros. unfold labNodes.
+  intros. unfold IG_basic_labNodes.
   rewrite In_map_fst_InA.
   pose proof (WF.elements_in_iff ig).
   rewrite In_conditions_same in H.
@@ -98,10 +94,10 @@ Qed.
 
 
 (* 5 statements on inserting (helpers for mkGraph): update, insEdge, insEdges, insNode, insNodes *)
-Lemma updateEntry_does_not_change_key_set : forall (node : Node) (f : NatSet.t * NatSet.t -> NatSet.t * NatSet.t) (ig : IG) (x : Node),
-  In x (labNodes (updateEntry node f ig)) <-> In x (labNodes ig).
+Lemma updateEntry_does_not_change_key_set : forall (node : Node) (f : NatSet.t * NatSet.t -> NatSet.t * NatSet.t) (ig : IG_basic) (x : Node),
+  In x (IG_basic_labNodes (_updateEntry node f ig)) <-> In x (IG_basic_labNodes ig).
 Proof.
-  intros. unfold updateEntry.
+  intros. unfold _updateEntry.
   destruct (NatMap.find (elt:=NatSet.t * NatSet.t) node ig) eqn:isIn.
   - rewrite In_labNodes_is_InMap. rewrite In_labNodes_is_InMap. rewrite WF.add_in_iff.
     rewrite WF.in_find_iff. split.
@@ -113,10 +109,10 @@ Proof.
 Qed.
 
 
-Lemma insEdge_does_not_add_node : forall (edge : (Node * Node)) (ig : IG) (x : Node),
-  In x (labNodes (insEdge edge ig)) <-> In x (labNodes ig).
+Lemma insEdge_does_not_add_node : forall (edge : (Node * Node)) (ig : IG_basic) (x : Node),
+  In x (IG_basic_labNodes (_insEdge edge ig)) <-> In x (IG_basic_labNodes ig).
 Proof.
-  intros. unfold insEdge. destruct edge.
+  intros. unfold _insEdge. destruct edge.
   destruct (NatMap.mem (elt:=NatSet.t * NatSet.t) n ig && NatMap.mem (elt:=NatSet.t * NatSet.t) n0 ig) eqn:H0.
   - rewrite updateEntry_does_not_change_key_set.
     rewrite updateEntry_does_not_change_key_set.
@@ -125,8 +121,8 @@ Proof.
 Qed.
 
 
-Lemma insEdges_does_not_add_nodes : forall (edges : list (Node * Node)) (ig : IG) (x : Node),
-  In x (labNodes (insEdges edges ig)) <-> In x (labNodes ig).
+Lemma insEdges_does_not_add_nodes : forall (edges : list (Node * Node)) (ig : IG_basic) (x : Node),
+  In x (IG_basic_labNodes (_insEdges edges ig)) <-> In x (IG_basic_labNodes ig).
 Proof.
   intros. simpl. induction edges.
   - simpl. reflexivity.
@@ -134,18 +130,18 @@ Proof.
 Qed. 
 
 
-Lemma insNode_any_ins_node : forall (node : Node) (ig : IG) (x : Node),
-  In x (labNodes (insNode node ig)) <-> In x (node :: labNodes ig).
+Lemma insNode_any_ins_node : forall (node : Node) (ig : IG_basic) (x : Node),
+  In x (IG_basic_labNodes (_insNode node ig)) <-> In x (node :: IG_basic_labNodes ig).
 Proof.
-  intros. simpl. unfold insNode.
+  intros. simpl. unfold _insNode.
   rewrite In_labNodes_is_InMap. rewrite WF.add_in_iff.
   rewrite In_labNodes_is_InMap.
   reflexivity.
 Qed.  
 
 
-Lemma insNodes_any_ins_all_nodes : forall (nodes : list Node) (ig : IG) (x : Node),
-  In x (labNodes (insNodes nodes ig)) <-> In x (nodes ++ labNodes ig).
+Lemma insNodes_any_ins_all_nodes : forall (nodes : list Node) (ig : IG_basic) (x : Node),
+  In x (IG_basic_labNodes (_insNodes nodes ig)) <-> In x (nodes ++ IG_basic_labNodes ig).
 Proof.
   intros. induction nodes.
     - simpl. reflexivity.
@@ -153,18 +149,18 @@ Proof.
 Qed.
 
 Lemma insEdge_on_empty_is_empty : forall (edge : Node * Node),
-  insEdge edge empty = empty.
+  _insEdge edge IG_basic_empty = IG_basic_empty.
 (* This proof is very similar to "insEdge_does_not_add_node", but using it here it is more complicated than just doing it again  *)
 Proof.
-  intros. unfold insEdge. destruct edge.
-  destruct (NatMap.mem (elt:=NatSet.t * NatSet.t) n empty && NatMap.mem (elt:=NatSet.t * NatSet.t) n0 empty) eqn:cond.
+  intros. unfold _insEdge. destruct edge.
+  destruct (NatMap.mem (elt:=NatSet.t * NatSet.t) n IG_basic_empty && NatMap.mem (elt:=NatSet.t * NatSet.t) n0 IG_basic_empty) eqn:cond.
   - compute. reflexivity.
   - reflexivity.
 Qed. 
 
 
 Lemma insEdges_on_empty_is_empty : forall (edges : list (Node * Node)),
-  insEdges edges empty = empty.
+  _insEdges edges IG_basic_empty = IG_basic_empty.
 (* This proof is very similar to "insEdges_does_not_add_nodes", but using it here it is more complicated than just doing it again  *)
 Proof.
   intros. induction edges; simpl.
@@ -176,19 +172,19 @@ Qed.
 
 (* "big" statement: *)
 Theorem mkGraph_any_ins_all_nodes : forall (nl : list Node) (el : list (Node * Node)) (x : Node),
-  In x (labNodes (mkGraph nl el)) <-> In x nl.
+  In x (IG_basic_labNodes (IG_basic_mkGraph nl el)) <-> In x nl.
 Proof.
-  intros. unfold mkGraph. rewrite insEdges_does_not_add_nodes. rewrite insNodes_any_ins_all_nodes.
+  intros. unfold IG_basic_mkGraph. rewrite insEdges_does_not_add_nodes. rewrite insNodes_any_ins_all_nodes.
   rewrite app_nil_r. reflexivity.
 Qed.
 
 
-Theorem empty_isEmpty : isEmpty empty = true.
+Theorem empty_isEmpty : IG_basic_isEmpty IG_basic_empty = true.
 Proof.
   compute. reflexivity.
 Qed.
 
-Theorem labNodes_empty_nil : labNodes empty = [].
+Theorem labNodes_empty_nil : IG_basic_labNodes IG_basic_empty = [].
 Proof.
   compute. reflexivity.
 Qed.
@@ -204,10 +200,10 @@ Qed.
 
 
 Theorem  non_empty_isEmpty_false : forall (nodes : list Node) (edges : list (Node * Node)),
-  length nodes <> 0 <-> isEmpty ((mkGraph nodes edges)) = false.
+  length nodes <> 0 <-> IG_basic_isEmpty ((IG_basic_mkGraph nodes edges)) = false.
 Proof.
-  intros. unfold isEmpty. rewrite <- not_NatMap_Empty_is_empty_false. unfold not.
-  destruct nodes; simpl; unfold mkGraph.
+  intros. unfold IG_basic_isEmpty. rewrite <- not_NatMap_Empty_is_empty_false. unfold not.
+  destruct nodes; simpl; unfold IG_basic_mkGraph.
   - firstorder.
     apply H.
     apply WP.elements_Empty.
@@ -234,21 +230,21 @@ Qed.
 
 
 
-Theorem matsh_empty_is_nothing : forall (node : Node), matsh node empty = (None, empty).
+Theorem matsh_empty_is_nothing : forall (node : Node), IG_basic_match node IG_basic_empty = (None, IG_basic_empty).
 Proof.
   intros. compute. reflexivity.
 Qed.
 
 
 Theorem spec4 : forall (node : Node) (nodes : list Node) (edges : list (Node * Node)), 
-  In node nodes -> exists froms tos, matsh node (mkGraph nodes edges) =
-  (Some (froms, tos), mkGraph (filter (fun n => negb (node =? n)) nodes) (filter (fun '(from, to) => negb ((from =? node) || (to =? node))) edges)).
+  In node nodes -> exists froms tos, IG_basic_match node (IG_basic_mkGraph nodes edges) =
+  (Some (froms, tos), IG_basic_mkGraph (filter (fun n => negb (node =? n)) nodes) (filter (fun '(from, to) => negb ((from =? node) || (to =? node))) edges)).
 (* This is not even a complete specification and it looks like a hard one to prove... *)
 Proof.
 Admitted.
 
 
 Theorem spec5 : forall (node : Node) (nodes : list Node) (edges : list (Node * Node)), 
-  not (In node nodes) -> matsh node (mkGraph nodes edges) = (None, mkGraph nodes edges).
+  not (In node nodes) -> IG_basic_match node (IG_basic_mkGraph nodes edges) = (None, IG_basic_mkGraph nodes edges).
 Proof.
 Admitted.
